Proved the refinement relation between the actual VM implementation and the ones with correctness proofs.

Regex/VM/Basic2.lean
@@ -6,55 +6,128 @@ set_option autoImplicit false
 
 open Regex.Data (SparseSet Vec)
 open Regex (NFA)
-open String (Pos)
+open String (Pos Iterator)
 
 namespace Regex.VM
 
--- `nfa.maxTag` is erased, so we don't need to traverse the whole nodes to use `Buffer`.
-def Buffer (nfa : NFA) := Vec (Option Pos) (nfa.maxTag + 1)
+abbrev Buffer (size : Nat) := Vec (Option Pos) size
+
+-- TODO: check if `mkArray`-based implementation is more efficient
+def Buffer.empty {size : Nat} : Buffer size := Vec.ofFn (fun _ => .none)
+
+structure SearchState (nfa : NFA) (bufferSize : Nat) where
+  states : SparseSet nfa.nodes.size
+  updates : Vec (Buffer bufferSize) nfa.nodes.size
+
+abbrev εStack (nfa : NFA) (bufferSize : Nat) := List (Buffer bufferSize × Fin nfa.nodes.size)
 
 /--
-The stack for εClosure. Each entry consists of a pair of an NFA state and the capture group buffer
-at that state.
--/
-abbrev εStack (nfa : NFA) := List (Buffer nfa × Fin nfa.nodes.size)
+Visit all ε-transitions from the states in the stack, updating `next.states` when the new state is
+`.done`, `.char`, or `.sparse`. Returns `.some buffer` if a `.done` state is reached, meaning a
+match is found.
 
--- TODO: System V ABI only supports at most 6 arguments in registers. Should we put `wf` as `Subtype` to reduce the number of arguments?
--- TODO: Windows even supports only 4 arguments in registers.
-def εClosure2 (nfa : NFA) (wf : nfa.WellFormed) (pos : Pos)
-  (next : SparseSet nfa.nodes.size) (matched : Option (Buffer nfa)) (buffers : Vec (Buffer nfa) nfa.nodes.size)
-  (stack : εStack nfa) :
-  (SparseSet nfa.nodes.size × Option (Buffer nfa) × Vec (Buffer nfa) nfa.nodes.size) :=
+The actual VM implementation tracks only the last write for each offset, materializing all updates
+as a buffer.
+-/
+def εClosure2 {bufferSize : Nat} (nfa : NFA) (wf : nfa.WellFormed) (it : Iterator)
+  (matched : Option (Buffer bufferSize)) (next : SearchState nfa bufferSize) (stack : εStack nfa bufferSize) :
+  Option (Buffer bufferSize) × SearchState nfa bufferSize :=
   match stack with
-  | [] => (next, matched, buffers)
-  | (buffer, state) :: stack' =>
-    if state ∈ next then
-      εClosure2 nfa wf pos next matched buffers stack'
+  | [] => (matched, next)
+  | (update, state) :: stack' =>
+    if state ∈ next.states then
+      εClosure2 nfa wf it matched next stack'
     else
-      let next' := next.insert state
+      let states' := next.states.insert state
       match hn : nfa[state] with
       | .epsilon state' =>
         have isLt : state' < nfa.nodes.size := wf.inBounds' state hn
-        εClosure2 nfa wf pos next' matched buffers ((buffer, ⟨state', isLt⟩) :: stack')
+        εClosure2 nfa wf it matched ⟨states', next.updates⟩ ((update, ⟨state', isLt⟩) :: stack')
       | .split state₁ state₂ =>
         have isLt : state₁ < nfa.nodes.size ∧ state₂ < nfa.nodes.size := wf.inBounds' state hn
-        εClosure2 nfa wf pos next' matched buffers ((buffer, ⟨state₁, isLt.1⟩) :: (buffer, ⟨state₂, isLt.2⟩):: stack')
+        εClosure2 nfa wf it matched ⟨states', next.updates⟩ ((update, ⟨state₁, isLt.1⟩) :: (update, ⟨state₂, isLt.2⟩):: stack')
       | .save offset state' =>
         have isLt : state' < nfa.nodes.size := wf.inBounds' state hn
-        have offsetLe := nfa.le_maxTag state hn
-        let buffer' := buffer.set offset (by omega) pos
-        εClosure2 nfa wf pos next' matched buffers ((buffer', ⟨state', isLt⟩) :: stack')
+        -- Write the position only when `offset` is in bounds.
+        let update' := update.setIfInBounds offset it.pos
+        εClosure2 nfa wf it matched ⟨states', next.updates⟩ ((update', ⟨state', isLt⟩) :: stack')
       | .done =>
-        let matched' := matched <|> buffer
-        let buffers' := buffers.set state state.isLt buffer
-        εClosure2 nfa wf pos next' matched' buffers' stack'
-      | .char _ _ =>
-        let buffers' := buffers.set state state.isLt buffer
-        εClosure2 nfa wf pos next' matched buffers' stack'
-      | .sparse _ _ =>
-        let buffers' := buffers.set state state.isLt buffer
-        εClosure2 nfa wf pos next' matched buffers' stack'
-      | .fail => εClosure2 nfa wf pos next' matched buffers stack'
-termination_by (next.measure, stack)
+        let matched' := matched <|> update
+        let updates' := next.updates.set state state.isLt update
+        εClosure2 nfa wf it matched' ⟨states', updates'⟩ stack'
+      | .char c state' =>
+        let updates' := next.updates.set state state.isLt update
+        εClosure2 nfa wf it matched ⟨states', updates'⟩ stack'
+      | .sparse cs state' =>
+        let updates' := next.updates.set state state.isLt update
+        εClosure2 nfa wf it matched ⟨states', updates'⟩ stack'
+      | .fail => εClosure2 nfa wf it matched ⟨states', next.updates⟩ stack'
+termination_by (next.states.measure, stack)
+
+/--
+If the given state can make a transition on the current character of `it`, make the transition and
+traverse ε-closures from the resulting state.
+-/
+def stepChar2 {bufferSize : Nat} (nfa : NFA) (wf : nfa.WellFormed) (it : Iterator) (currentUpdates : Vec (Buffer bufferSize) nfa.nodes.size)
+  (next : SearchState nfa bufferSize) (state : Fin nfa.nodes.size) :
+  Option (Buffer bufferSize) × SearchState nfa bufferSize :=
+  match hn : nfa[state] with
+  | .char c state' =>
+    if it.curr = c then
+      have isLt := wf.inBounds' state hn
+      let update := currentUpdates.get state state.isLt
+      εClosure2 nfa wf it.next .none next [(update, ⟨state', isLt⟩)]
+    else
+      (.none, next)
+  | .sparse cs state' =>
+    if it.curr ∈ cs then
+      have isLt := wf.inBounds' state hn
+      let update := currentUpdates.get state state.isLt
+      εClosure2 nfa wf it.next .none next [(update, ⟨state', isLt⟩)]
+    else
+      (.none, next)
+  | _ => (.none, next)
+
+/--
+For all states in `current`, make a transition on the current character of `it` and traverse
+ε-closures from the resulting states.
+-/
+def eachStepChar2 {bufferSize : Nat} (nfa : NFA) (wf : nfa.WellFormed) (it : Iterator)
+  (current : SearchState nfa bufferSize) (next : SearchState nfa bufferSize) :
+  Option (Buffer bufferSize) × SearchState nfa bufferSize :=
+  go 0 (Nat.zero_le _) next
+where
+  go (i : Nat) (hle : i ≤ current.states.count) (next : SearchState nfa bufferSize) :
+    Option (Buffer bufferSize) × SearchState nfa bufferSize :=
+    if h : i = current.states.count then
+      (.none, next)
+    else
+      have hlt : i < current.states.count := Nat.lt_of_le_of_ne hle h
+      let result := stepChar2 nfa wf it current.updates next current.states[i]
+      if result.1.isSome then
+        result
+      else
+        go (i + 1) hlt result.2
+
+def captureNext2 (nfa : NFA) (wf : nfa.WellFormed) (bufferSize : Nat) (it : Iterator) : Option (Buffer bufferSize) :=
+  let updates : Vec (Buffer bufferSize) nfa.nodes.size := Vec.ofFn (fun _ => Buffer.empty)
+  let (matched, current) := εClosure2 nfa wf it .none ⟨.empty, updates⟩ [(Buffer.empty, ⟨nfa.start, wf.start_lt⟩)]
+  go it matched current ⟨.empty, updates⟩
+where
+  go (it : Iterator) (matched : Option (Buffer bufferSize)) (current next : SearchState nfa bufferSize) :
+    Option (Buffer bufferSize) :=
+    if it.atEnd then
+      matched
+    else
+      if current.states.isEmpty && matched.isSome then
+        matched
+      else
+        if matched.isNone then
+          let expanded := εClosure2 nfa wf it .none current [(Buffer.empty, ⟨nfa.start, wf.start_lt⟩)]
+          let stepped := eachStepChar2 nfa wf it expanded.2 next
+          go it.next stepped.1 stepped.2 ⟨current.states.clear, current.updates⟩
+        else
+          let stepped := eachStepChar2 nfa wf it current next
+          go it.next (stepped.1 <|> matched) stepped.2 ⟨current.states.clear, current.updates⟩
 
 end Regex.VM
