RegexCorrectness/VM/Correspondence/Refinement/Refinement.lean
@@ -1,0 +1,336 @@
+import RegexCorrectness.VM.Search
+import RegexCorrectness.VM.Correspondence.Materialize
+import RegexCorrectness.VM.Correspondence.Refinement.Simp
+
+set_option autoImplicit false
+
+open Regex.Data (SparseSet Vec)
+open Regex (NFA)
+open Regex.NFA (materializeUpdates)
+open String (Pos Iterator)
+
+/-
+The correctness proofs use the refined versions of the VM functions to track all updates to the
+capture groups while the actual implementation tracks only the last update per capture group.
+
+This files estabilishes the correspondence between the refined and actual VM functions.
+-/
+namespace Regex.VM
+
+variable {nfa : NFA} {wf : nfa.WellFormed} {bufferSize : Nat} {it : Iterator}
+  {matched : Option (Buffer bufferSize)} {matched' : Option (List (Nat × Pos))}
+  {next : SearchState nfa bufferSize} {next' : SearchState' nfa}
+  {stack : εStack nfa bufferSize} {stack' : εStack' nfa}
+
+def refineUpdate (update : List (Nat × Pos)) (buffer : Buffer bufferSize) : Prop :=
+  materializeUpdates bufferSize update = buffer
+
+@[simp]
+theorem refineUpdate.empty : @refineUpdate bufferSize [] Buffer.empty := rfl
+
+def refineUpdateOpt : Option (List (Nat × Pos)) → Option (Buffer bufferSize) → Prop
+  | .none, .none => True
+  | .some update, .some buffer => refineUpdate update buffer
+  | _, _ => False
+
+theorem refineUpdateOpt.isSome_iff (h : refineUpdateOpt matched' matched) :
+  matched'.isSome ↔ matched.isSome := by
+  match matched', matched with
+  | .none, .none => simp
+  | .some _, .some _ => simp
+  | .none, .some _ | .some _, .none => simp [refineUpdateOpt] at h
+
+theorem refineUpdateOpt.isNone_iff (h : refineUpdateOpt matched' matched) :
+  matched'.isNone ↔ matched.isNone := by
+  match matched', matched with
+  | .none, .none => simp
+  | .some _, .some _ => simp
+  | .none, .some _ | .some _, .none => simp [refineUpdateOpt] at h
+
+theorem refineUpdateOpt.orElse {update₁ update₂ : Option (List (Nat × Pos))} {buffer₁ buffer₂ : Option (Buffer bufferSize)}
+  (h₁ : refineUpdateOpt update₁ buffer₁) (h₂ : refineUpdateOpt update₂ buffer₂) :
+  refineUpdateOpt (update₁ <|> update₂) (buffer₁ <|> buffer₂) := by
+  match update₁, buffer₁ with
+  | .some _, .some _ => simp [h₁]
+  | .none, .none => simp [h₂]
+  | .none, .some _ | .some _, .none => simp [refineUpdateOpt] at h₁
+
+def refineUpdates (updates : Vec (List (Nat × Pos)) nfa.nodes.size) (buffers : Vec (Buffer bufferSize) nfa.nodes.size) : Prop :=
+  ∀ (i : Fin nfa.nodes.size), refineUpdate updates[i] buffers[i]
+
+def SearchState'.refines (state' : SearchState' nfa) (state : SearchState nfa bufferSize) : Prop :=
+  state'.states = state.states ∧ refineUpdates state'.updates state.updates
+
+inductive εStack'.refines : εStack' nfa → εStack nfa bufferSize → Prop where
+  | nil : εStack'.refines [] []
+  | cons {update state' tail' buffer state tail}
+    (h₁ : materializeUpdates bufferSize update = buffer) (h₂ : state' = state) (rest : εStack'.refines tail' tail) :
+    εStack'.refines ((update, state') :: tail') ((buffer, state) :: tail)
+
+@[simp]
+theorem εStack'.refines_nil : εStack'.refines [] stack ↔ stack = [] :=
+  ⟨fun ref => by cases ref; simp, fun h => h ▸ .nil⟩
+
+@[simp]
+theorem εStack'.refines_cons {update state' tail' stack} :
+  @εStack'.refines nfa bufferSize ((update, state') :: tail') stack ↔
+  ∃ buffer state tail, stack = (buffer, state) :: tail ∧ materializeUpdates bufferSize update = buffer ∧ state' = state ∧ @εStack'.refines nfa bufferSize tail' tail := by
+  apply Iff.intro
+  . intro ref
+    cases ref with
+    | cons h₁ h₂ rest => exact ⟨_, _, _, rfl, h₁, h₂, rest⟩
+  . intro ⟨buffer, state, tail, eq, h₁, h₂, rest⟩
+    exact eq ▸ .cons h₁ h₂ rest
+
+theorem εClosure'.refines {result result'}
+  (h : εClosure2 nfa wf it matched next stack = result)
+  (h' : εClosure' nfa wf it matched' next' stack' = result')
+  (refMatched : refineUpdateOpt matched' matched)
+  (refState : next'.refines next)
+  (refStack : stack'.refines stack) :
+  refineUpdateOpt result'.1 result.1 ∧ result'.2.refines result.2 := by
+  induction matched', next', stack' using εClosure'.induct' nfa wf it generalizing matched next stack result result' with
+  | base matched' next' =>
+    simp at refStack
+    subst stack
+    simp at h' h
+    simp [←h', ←h, refMatched, refState]
+  | visited matched' next' update state' stack' mem ih =>
+    cases refStack with
+    | @cons _ _ tail' buffer state tail h₁ h₂ rest =>
+      rw [εClosure'_visited mem] at h'
+      rw [εClosure_visited (refState.1 ▸ h₂ ▸ mem)] at h
+      exact ih h h' refMatched refState rest
+  | epsilon matched' next' update state' stack' state mem hn next'' =>
+    -- TODO: cannot introduce `ih` directly for some reason
+    rename_i ih
+    cases refStack with
+    | @cons _ _ tail' buffer state tail h₁ h₂ rest =>
+      rw [εClosure'_epsilon mem hn] at h'
+      rw [εClosure_epsilon (refState.1 ▸ h₂ ▸ mem) (h₂ ▸ hn)] at h
+      have : next''.refines ⟨next.states.insert state, next.updates⟩ := by
+        simp [SearchState'.refines, h₂, refState.1]
+        exact refState.2
+      exact ih h h' refMatched this (.cons h₁ rfl rest)
+  | split matched' next' update state stack' state₁ state₂ mem hn next'' =>
+    rename_i ih
+    cases refStack with
+    | @cons _ _ tail' buffer state tail h₁ h₂ rest =>
+      rw [εClosure'_split mem hn] at h'
+      rw [εClosure_split (refState.1 ▸ h₂ ▸ mem) (h₂ ▸ hn)] at h
+      have : next''.refines ⟨next.states.insert state, next.updates⟩ := by
+        simp [SearchState'.refines, h₂, refState.1]
+        exact refState.2
+      exact ih h h' refMatched this (.cons h₁ rfl (.cons h₁ rfl rest))
+  | save matched' next' update state stack' offset state' mem hn next'' =>
+    rename_i ih
+    cases refStack with
+    | @cons _ _ tail' buffer state tail h₁ h₂ rest =>
+      rw [εClosure'_save mem hn] at h'
+      rw [εClosure_save (refState.1 ▸ h₂ ▸ mem) (h₂ ▸ hn)] at h
+      have : next''.refines ⟨next.states.insert state, next.updates⟩ := by
+        simp [SearchState'.refines, h₂, refState.1]
+        exact refState.2
+      exact ih h h' refMatched this (.cons (by simp [h₁]) rfl rest)
+  | done matched' next' update state stack' mem hn next'' =>
+    rename_i ih
+    cases refStack with
+    | @cons _ _ tail' buffer state tail h₁ h₂ rest =>
+      rw [εClosure'_done mem hn] at h'
+      rw [εClosure_done (refState.1 ▸ h₂ ▸ mem) (h₂ ▸ hn)] at h
+      have refMatched' : refineUpdateOpt (matched' <|> some update) (matched <|> some buffer) :=
+        refineUpdateOpt.orElse refMatched h₁
+      have : next''.refines ⟨next.states.insert state, next.updates.set state state.isLt buffer⟩ := by
+        simp [SearchState'.refines, h₂, refState.1]
+        intro i
+        if h : state = i then
+          simp [h]
+          exact h₁
+        else
+          have : state.val ≠ i := Fin.val_ne_of_ne h
+          simp [this]
+          exact refState.2 i
+      exact ih h h' refMatched' this rest
+  | char matched' next' update state stack' c state' mem hn next'' =>
+    rename_i ih
+    cases refStack with
+    | @cons _ _ tail' buffer state tail h₁ h₂ rest =>
+      rw [εClosure'_char mem hn] at h'
+      rw [εClosure_char (refState.1 ▸ h₂ ▸ mem) (h₂ ▸ hn)] at h
+      have : next''.refines ⟨next.states.insert state, next.updates.set state state.isLt buffer⟩ := by
+        simp [SearchState'.refines, h₂, refState.1]
+        intro i
+        if h : state = i then
+          simp [h]
+          exact h₁
+        else
+          have : state.val ≠ i := Fin.val_ne_of_ne h
+          simp [this]
+          exact refState.2 i
+      exact ih h h' refMatched this rest
+  | sparse matched' next' update state stack' cs state' mem hn next'' =>
+    rename_i ih
+    cases refStack with
+    | @cons _ _ tail' buffer state tail h₁ h₂ rest =>
+      rw [εClosure'_sparse mem hn] at h'
+      rw [εClosure_sparse (refState.1 ▸ h₂ ▸ mem) (h₂ ▸ hn)] at h
+      have : next''.refines ⟨next.states.insert state, next.updates.set state state.isLt buffer⟩ := by
+        simp [SearchState'.refines, h₂, refState.1]
+        intro i
+        if h : state = i then
+          simp [h]
+          exact h₁
+        else
+          have : state.val ≠ i := Fin.val_ne_of_ne h
+          simp [this]
+          exact refState.2 i
+      exact ih h h' refMatched this rest
+  | fail matched' next' update state stack' mem hn next'' =>
+    rename_i ih
+    cases refStack with
+    | @cons _ _ tail' buffer state tail h₁ h₂ rest =>
+      rw [εClosure'_fail mem hn] at h'
+      rw [εClosure_fail (refState.1 ▸ h₂ ▸ mem) (h₂ ▸ hn)] at h
+      have : next''.refines ⟨next.states.insert state, next.updates⟩ := by
+        simp [SearchState'.refines, h₂, refState.1]
+        exact refState.2
+      exact ih h h' refMatched this rest
+
+theorem stepChar'.refines {currentUpdates currentUpdates' state result result'}
+  (h : stepChar2 nfa wf it currentUpdates next state = result)
+  (h' : stepChar' nfa wf it currentUpdates' next' state = result')
+  (refUpdates : refineUpdates currentUpdates' currentUpdates)
+  (refState : next'.refines next) :
+  refineUpdateOpt result'.1 result.1 ∧ result'.2.refines result.2 := by
+  unfold stepChar' at h'
+  split at h'
+  next c state' hn =>
+    rw [stepChar_char hn] at h
+    split at h'
+    next eq =>
+      simp [eq] at h h'
+      exact εClosure'.refines h h' (by simp [refineUpdateOpt]) refState (.cons (refUpdates state) rfl .nil)
+    next ne =>
+      simp [ne] at h
+      simp [←h', ←h, refineUpdateOpt, refState]
+  next cs state' hn =>
+    rw [stepChar_sparse hn] at h
+    split at h'
+    next mem =>
+      simp [mem] at h h'
+      exact εClosure'.refines h h' (by simp [refineUpdateOpt]) refState (.cons (refUpdates state) rfl .nil)
+    next nmem =>
+      simp [nmem] at h
+      simp [←h', ←h, refineUpdateOpt, refState]
+  next h₁ h₂ =>
+    rw [stepChar_not_char_sparse h₁ h₂] at h
+    simp [←h', ←h, refineUpdateOpt, refState]
+
+theorem eachStepChar'.go.refines {current current' i hle hle' result result'}
+  (h : eachStepChar2.go nfa wf it current i hle next = result)
+  (h' : eachStepChar'.go nfa wf it current' i hle' next' = result')
+  (refCurrent : current'.refines current)
+  (refNext : next'.refines next) :
+  refineUpdateOpt result'.1 result.1 ∧ result'.2.refines result.2 := by
+  induction i, hle', next' using eachStepChar'.go.induct' nfa wf it generalizing current next result result' with
+  | base next' =>
+    simp at h'
+    simp [refCurrent.1] at h
+    simp [←h', ←h, refineUpdateOpt, refNext]
+  | found i hlt' next' matched' next'' hstep' isSome' =>
+    have hlt : i < current.states.count := refCurrent.1 ▸ hlt'
+    have eq : current.states[i] = current'.states[i] := by
+      simp [refCurrent.1]
+    generalize hstep : stepChar2 nfa wf it current.updates next current.states[i] = stepped
+    have refStepChar := stepChar'.refines hstep (eq ▸ hstep') refCurrent.2 refNext
+    simp at refStepChar
+    have isSome : stepped.1.isSome := by
+      simp [refineUpdateOpt.isSome_iff refStepChar.1] at isSome'
+      exact isSome'
+    rw [eachStepChar'.go_found hlt' hstep' isSome'] at h'
+    rw [eachStepChar.go_found hlt hstep isSome] at h
+    simp [←h', ←h, refStepChar]
+  | not_found i hlt' next' matched' next'' hstep' isSome' ih =>
+    have hlt : i < current.states.count := refCurrent.1 ▸ hlt'
+    have eq : current.states[i] = current'.states[i] := by
+      simp [refCurrent.1]
+    generalize hstep : stepChar2 nfa wf it current.updates next current.states[i] = stepped
+    have refStepChar := stepChar'.refines hstep (eq ▸ hstep') refCurrent.2 refNext
+    simp at refStepChar
+    have isSome : ¬stepped.1.isSome := by
+      rw [refineUpdateOpt.isSome_iff refStepChar.1] at isSome'
+      exact isSome'
+    rw [eachStepChar'.go_not_found hlt' hstep' isSome'] at h'
+    rw [eachStepChar.go_not_found hlt hstep isSome] at h
+    exact ih h h' refCurrent refStepChar.2
+
+theorem eachStepChar'.refines {current current' result result'}
+  (h : eachStepChar2 nfa wf it current next = result)
+  (h' : eachStepChar' nfa wf it current' next' = result')
+  (refCurrent : current'.refines current)
+  (refNext : next'.refines next) :
+  refineUpdateOpt result'.1 result.1 ∧ result'.2.refines result.2 :=
+  eachStepChar'.go.refines h h' refCurrent refNext
+
+theorem captureNext'.go.refines {current current' result result'}
+  (h : captureNext2.go nfa wf bufferSize it matched current next = result)
+  (h' : captureNext'.go nfa wf it matched' current' next' = result')
+  (refMatched : refineUpdateOpt matched' matched)
+  (refCurrent : current'.refines current)
+  (refNext : next'.refines next) :
+  refineUpdateOpt result' result := by
+  induction it, matched', current', next' using captureNext'.go.induct' nfa wf generalizing matched current next result result' with
+  | not_found it matched' current' next' atEnd =>
+    rw [captureNext'.go_not_found atEnd] at h'
+    rw [captureNext.go_not_found atEnd] at h
+    simp [←h', ←h, refMatched]
+  | found it matched' current' next' atEnd isEmpty' isSome' =>
+    have isEmpty : current.states.isEmpty := refCurrent.1 ▸ isEmpty'
+    have isSome : matched.isSome := by
+      rw [refineUpdateOpt.isSome_iff refMatched] at isSome'
+      exact isSome'
+    rw [captureNext'.go_found atEnd isEmpty' isSome'] at h'
+    rw [captureNext.go_found atEnd isEmpty isSome] at h
+    simp [←h', ←h, refMatched]
+  | ind_not_found it matched' current' next' _ current'' matched'' next'' atEnd isNone' h₁ h₂ ih =>
+    have isNone : matched.isNone := by
+      rw [refineUpdateOpt.isNone_iff refMatched] at isNone'
+      exact isNone'
+    generalize hexpand : εClosure2 nfa wf it .none current [(Buffer.empty, ⟨nfa.start, wf.start_lt⟩)] = expanded
+    generalize hstep : eachStepChar2 nfa wf it expanded.2 next = stepped
+    rw [captureNext'.go_ind_not_found atEnd isNone' h₁ h₂] at h'
+    rw [captureNext.go_ind_not_found atEnd isNone hexpand hstep] at h
+
+    have := εClosure'.refines hexpand h₁ (by simp [refineUpdateOpt]) refCurrent (.cons rfl rfl .nil)
+    simp at this
+    have ⟨refMatched'', refNext''⟩ := eachStepChar'.refines hstep h₂ this.2 refNext
+    simp at refMatched'' refNext''
+    exact ih h h' refMatched'' refNext'' (by simp [refCurrent.1, SearchState'.refines, refCurrent.2])
+  | ind_found it matched' current' next' matched'' next'' atEnd isEmpty' isSome' h'' ih =>
+    have isEmpty : ¬current.states.isEmpty := refCurrent.1 ▸ isEmpty'
+    have isSome : matched.isSome := by
+      rw [refineUpdateOpt.isSome_iff refMatched] at isSome'
+      exact isSome'
+    generalize hstep : eachStepChar2 nfa wf it current next = stepped
+    rw [captureNext'.go_ind_found atEnd isEmpty' isSome' h''] at h'
+    rw [captureNext.go_ind_found atEnd isEmpty isSome hstep] at h
+
+    have := eachStepChar'.refines hstep h'' refCurrent refNext
+    simp at this
+    have ⟨refMatched'', refNext''⟩ := this
+    have : refineUpdateOpt (matched'' <|> matched') (stepped.1 <|> matched) :=
+      refineUpdateOpt.orElse refMatched'' refMatched
+    exact ih h h' this refNext'' (by simp [refCurrent.1, SearchState'.refines, refCurrent.2])
+
+theorem captureNext'.refines :
+  refineUpdateOpt (captureNext' nfa wf it) (captureNext2 nfa wf bufferSize it) := by
+  unfold captureNext' captureNext2
+  simp
+  generalize hexpand' : εClosure' nfa wf it .none ⟨.empty, Vec.ofFn (fun _ => [])⟩ [([], ⟨nfa.start, wf.start_lt⟩)] = expanded'
+  generalize hexpand : εClosure2 nfa wf it .none ⟨.empty, Vec.ofFn (fun _ => Buffer.empty)⟩ [(Buffer.empty, ⟨nfa.start, wf.start_lt⟩)] = expanded
+
+  have ⟨refMatched, refState⟩ := εClosure'.refines hexpand hexpand'
+    (by simp [refineUpdateOpt]) (by simp [SearchState'.refines, refineUpdates]) (.cons rfl rfl .nil)
+  exact captureNext'.go.refines rfl rfl refMatched refState (by simp [SearchState'.refines, refineUpdates])
+
+end Regex.VM
